theories/Validity/Validity.v
@@ -18,12 +18,33 @@ Ltac substitution := eauto with substitution.
   substitution equality is eqSubst.
   One should think of VRel as a functional relation taking two arguments Γ, Γ'
   and returning eqSubst as an output *)
+  Inductive Fequiv L L' : Set := Fequiv_make : L ≤ε L' -> L' ≤ε L -> Fequiv L L'.
+  Notation "L =ε L'" := (Fequiv L L').
+  Instance Equivalence_Fequiv : Equivalence Fequiv.
+  Proof.
+    split.
+    + split; eapply Fwk_id.
+    + intros ?? []; now split.
+    + intros ??? [] []; split; now eapply Fwk_compose.
+  Qed.
+
+  Definition lFwk {L L'} (eq : L =ε L') : L ≤ε L'.
+  Proof. apply eq. Qed.
+
+  Definition rFwk {L L'} (eq : L =ε L') : L' ≤ε L.
+  Proof. apply eq. Qed.
+
+  Lemma Fequiv_Fup {L L'} {b} (eq : L =ε L') {new : newnat L} {new' : newnat L'} :
+   new = new' :> nat -> (Fcons' L' new' b) =ε (Fcons' L new b).
+  Proof.
+    destruct eq.
+    intros e; split; eapply Fwk_Fup; tea.
+    now symmetry.
+  Qed.
 
   Definition VRel@{i j | i < j +} `{ta : tag} `{!WfContext ta} :=
-  forall
-    (Γ Γ' : context)
-    (* (validSubst : forall (Δ : context) (σ : nat -> term) (wfΔ : [|- Δ]), Type@{i}) *)
-    (eqSubst : forall (Δ : context) (wfΔ : [|- Δ ]) (ρF : Γ ≤ε Δ) (ρF' : Γ' ≤ε Δ ) (σ σ' : nat -> term) , Type@{i})
+  forall (Γ Γ' : context)
+    (eqSubst : forall (Δ : context) (wfΔ : [|- Δ ]) (σ σ' : nat -> term) , Type@{i})
     , Type@{j}.
 
 (* A VPack contains the data corresponding to the codomain of VRel seen as a functional relation *)
@@ -32,8 +53,7 @@ Module VPack.
 
   Record VPack@{i} `{ta : tag} `{!WfContext ta} {Γ Γ' : context} :=
   {
-    (* validSubst : forall (Δ : context) (σ : nat -> term) (wfΔ : [|- Δ]), Type@{i} ; *)
-    eqSubst : forall (Δ : context) (wfΔ : [|- Δ ]) (ρF : Γ ≤ε Δ) (ρF' : Γ' ≤ε Δ ) (σ σ' : nat -> term) , Type@{i} ;
+    eqSubst : forall (Δ : context) (wfΔ : [|- Δ ]) (σ σ' : nat -> term) , Type@{i} ;
   }.
 
   Arguments VPack : clear implicits.
@@ -43,10 +63,10 @@ End VPack.
 
 Export VPack(VPack,Build_VPack).
 
-Notation "[ P | Δ ||-v σ : Γ | wfΔ ]" := (VPack.eqSubst (Γ:=Γ) P Δ wfΔ _ _ σ σ) (at level 0, P, Δ, σ, Γ, wfΔ at level 50).
-Notation "[ P | Δ ||-v σ : Γ ≅ Γ' | wfΔ ]" := (VPack.eqSubst (Γ:=Γ) (Γ':=Γ') P Δ wfΔ _ _ σ σ) (at level 0, P, Δ, σ, Γ, Γ', wfΔ at level 50).
-Notation "[ P | Δ ||-v σ ≅ σ' : Γ | wfΔ ]" := (VPack.eqSubst (Γ:=Γ) P Δ wfΔ _ _ σ σ') (at level 0, P, Δ, σ, σ', Γ, wfΔ at level 50).
-Notation "[ P | Δ ||-v σ ≅ σ' : Γ ≅ Γ' | wfΔ ]" := (VPack.eqSubst (Γ:=Γ) (Γ':=Γ') P Δ wfΔ _ _ σ σ') (at level 0, P, Δ, σ, σ', Γ, Γ', wfΔ at level 50).
+Notation "[ P | Δ ||-v σ : Γ | wfΔ ]" := (VPack.eqSubst (Γ:=Γ) P Δ wfΔ σ σ) (at level 0, P, Δ, σ, Γ, wfΔ at level 50).
+Notation "[ P | Δ ||-v σ : Γ ≅ Γ' | wfΔ ]" := (VPack.eqSubst (Γ:=Γ) (Γ':=Γ') P Δ wfΔ σ σ) (at level 0, P, Δ, σ, Γ, Γ', wfΔ at level 50).
+Notation "[ P | Δ ||-v σ ≅ σ' : Γ | wfΔ ]" := (VPack.eqSubst (Γ:=Γ) P Δ wfΔ σ σ') (at level 0, P, Δ, σ, σ', Γ, wfΔ at level 50).
+Notation "[ P | Δ ||-v σ ≅ σ' : Γ ≅ Γ' | wfΔ ]" := (VPack.eqSubst (Γ:=Γ) (Γ':=Γ') P Δ wfΔ σ σ') (at level 0, P, Δ, σ, σ', Γ, Γ', wfΔ at level 50).
 
 (* An VPack it adequate wrt. a VRel when its three unpacked components are *)
 #[universes(polymorphic)] Definition VPackAdequate@{i j} `{ta : tag} `{!WfContext ta}
@@ -77,8 +97,23 @@ Coercion VAd.adequate : VAdequate >-> VPackAdequate.
 
 Notation "[ R | ||-v Γ ]"                            := (VAdequate R Γ Γ) (at level 0, R, Γ at level 50).
 Notation "[ R | ||-v Γ ≅ Γ' ]"                       := (VAdequate R Γ Γ') (at level 0, R, Γ, Γ' at level 50).
-Notation "[ R | Δ ||-v σ : Γ | RΓ | wfΔ ]"           := (RΓ.(@VAd.pack _ _ R Γ _).(VPack.eqSubst) Δ wfΔ _ _ σ σ) (at level 0, R, Δ, σ, Γ, RΓ, wfΔ at level 50).
-Notation "[ R | Δ ||-v σ ≅ σ' : Γ | RΓ | wfΔ ]" := (RΓ.(@VAd.pack _ _ R Γ _).(VPack.eqSubst) Δ  wfΔ _ _ σ σ') (at level 0, R, Δ, σ, σ', Γ, RΓ, wfΔ at level 50).
+Notation "[ R | Δ ||-v σ : Γ | RΓ | wfΔ ]"           := (RΓ.(@VAd.pack _ _ R Γ _).(VPack.eqSubst) Δ wfΔ σ σ) (at level 0, R, Δ, σ, Γ, RΓ, wfΔ at level 50).
+Notation "[ R | Δ ||-v σ ≅ σ' : Γ | RΓ | wfΔ ]" := (RΓ.(@VAd.pack _ _ R Γ _).(VPack.eqSubst) Δ  wfΔ σ σ') (at level 0, R, Δ, σ, σ', Γ, RΓ, wfΔ at level 50).
+
+Record StypeValidity@{u i j k l} `{ta : tag} `{!WfContext ta}
+  `{!WfType ta} `{!Typing ta} `{!ConvType ta}
+  `{!ConvTerm ta} `{!ConvNeuConv ta} `{!RedType ta} `{!RedTerm ta}
+  {Γ Γ' : context} {VΓ : VPack@{u} Γ Γ'}
+  {l : TypeLevel} {A A' : term} :=
+  {
+    SvalidTyExt : forall {Δ : context} (wfΔ : [|- Δ ])
+      {σ σ' : nat -> term}
+      (vσσ' : [ VΓ | Δ ||-v σ ≅ σ' : Γ | wfΔ ])
+      , [LogRel@{i j k l} l | Δ ||- A [ σ ] ≅ A' [ σ' ] ]
+  }.
+
+Arguments StypeValidity : clear implicits.
+Arguments StypeValidity {_ _ _ _ _ _ _ _ _}.
 
 Record typeValidity@{u i j k l} `{ta : tag} `{!WfContext ta}
   `{!WfType ta} `{!Typing ta} `{!ConvType ta}
@@ -86,21 +121,35 @@ Record typeValidity@{u i j k l} `{ta : tag} `{!WfContext ta}
   {Γ Γ' : context} {VΓ : VPack@{u} Γ Γ'}
   {l : TypeLevel} {A A' : term} :=
   {
-    validTyExt : forall {Δ : context} (wfΔ : [|- Δ ]) {ρF : Γ ≤ε Δ} {ρF' : Γ' ≤ε Δ}
+    validTyExt : forall {Δ : context} (wfΔ : [|- Δ ])
       {σ σ' : nat -> term}
-      (vσσ' : [ VΓ | Δ ||-v σ ≅ σ' : Γ | wfΔ ])
-      , [LogRel@{i j k l} l | Δ ||- A [ σ ] ≅ A' [ σ' ] ]
+      (vσσ' : [ VΓ | Δ ||-v σ ≅ σ' : Γ | wfΔ ]),
+      WLRAdequate@{i j k l} Δ wfΔ l A[σ] A'[σ']
   }.
 
 Arguments typeValidity : clear implicits.
 Arguments typeValidity {_ _ _ _ _ _ _ _ _}.
 
+Notation "[ P | Γ ||-vS< l > A ≅ B ]" := (StypeValidity Γ _ P l A B) (at level 0, P, Γ, l, A, B at level 50).
 Notation "[ P | Γ ||-v< l > A ≅ B ]" := (typeValidity Γ _ P l A B) (at level 0, P, Γ, l, A, B at level 50).
 
-Definition emptyEqSubst@{u} `{ta : tag} `{!WfContext ta} {L L'}:
-  forall (Δ : context) (wfΔ : [|- Δ]) (ρF : L ≤ε Δ) (ρF': L' ≤ε Δ) (σ σ' : nat -> term), Type@{u} := fun _ _ _ _ _ _ => unit.
-Definition emptyVPack `{ta : tag} `{!WfContext ta} {L L'}: VPack (fromFctx L) (fromFctx L') :=
-  Build_VPack _ _ emptyEqSubst.
+Lemma validTy_return `{GenericTypingProperties} {Γ Γ'} {VΓ : VPack Γ Γ'} {l A B} :
+  [ VΓ | Γ ||-vS< l > A ≅ B ] -> [ VΓ | Γ ||-v< l > A ≅ B ].
+Proof.
+  intros vAB.
+  constructor.
+  intros.
+  eapply WAd_return.
+  now eapply vAB.
+Qed.
+
+
+Inductive emptyEqSubst@{u} `{ta : tag} `{!WfContext ta} (L L' : Fcontext) (eq : L =ε L')
+  (Δ : context) (wfΔ : [|- Δ]) (σ σ' : nat -> term): Type@{u} :=
+    eqleq (ρε : Δ ≤ε L).
+
+Definition emptyVPack `{ta : tag} `{!WfContext ta} {L L'} (eq : L =ε L'): VPack (fromFctx L) (fromFctx L') :=
+  Build_VPack _ _ (emptyEqSubst L L' eq).
 
 Section snocValid.
   Universe u i j k l.
@@ -108,14 +157,13 @@ Section snocValid.
   `{!WfType ta} `{!Typing ta} `{!ConvType ta}
   `{!ConvTerm ta} `{!ConvNeuConv ta} `{!RedType ta} `{!RedTerm ta}
   {Γ Γ': context} {VΓ : VPack@{u} Γ Γ'} {A A' : term} {l : TypeLevel}
-  {vA : typeValidity@{u i j k l} Γ Γ' VΓ l A A' (* [ VΓ | Γ ||-v< l > A ] *)}.
+  {vA : StypeValidity@{u i j k l} Γ Γ' VΓ l A A' (* [ VΓ | Γ ||-v< l > A ] *)}.
 
 
-
-  Record snocEqSubst {Δ : context} {wfΔ : [|- Δ]} (ρF : (Γ,,A) ≤ε Δ) (ρF : (Γ',,A') ≤ε Δ) {σ σ' : nat -> term} : Type :=
+  Record snocEqSubst {Δ : context} {wfΔ : [|- Δ]} {σ σ' : nat -> term} : Type :=
     {
       eqTail : [ VΓ | Δ ||-v ↑ >> σ ≅ ↑ >> σ' : Γ | wfΔ ] ;
-      eqHead : [ Δ ||-< l > σ var_zero ≅ σ' var_zero : A[↑ >> σ] | validTyExt vA wfΔ eqTail ]
+      eqHead : [ Δ ||-S< l > σ var_zero ≅ σ' var_zero : A[↑ >> σ] | SvalidTyExt vA wfΔ eqTail ]
     }.
 
   Definition snocVPack := Build_VPack@{u (* max(u,k) *)} (Γ ,, A) (Γ',,A') (@snocEqSubst).
@@ -133,11 +181,11 @@ Inductive VR@{i j k l} `{ta : tag}
   `{WfContext ta} `{WfType ta} `{Typing ta}
   `{ConvType ta} `{ConvTerm ta} `{ConvNeuConv ta}
   `{RedType ta} `{RedTerm ta} : VRel@{k l} :=
-  | VREmpty {L L'}: VR (fromFctx L) (fromFctx L') emptyEqSubst@{k}
+  | VREmpty {L L'} (eq : L =ε L') : VR (fromFctx L) (fromFctx L') (emptyEqSubst@{k} L L' eq)
   | VRSnoc : forall {Γ Γ':context} {A A' l}
     (VΓ : VPack@{k} Γ Γ')
     (VΓad : VPackAdequate@{k l} VR VΓ)
-    (VA : typeValidity@{k i j k l} Γ Γ' VΓ l A A' (*[ VΓ | Γ ||-v< l > A ]*)),
+    (VA : StypeValidity@{k i j k l} Γ Γ' VΓ l A A' (*[ VΓ | Γ ||-v< l > A ]*)),
     VR (Γ,,A) (Γ',,A') (snocEqSubst Γ Γ' VΓ A A' l VA).
 
 
@@ -147,30 +195,56 @@ Notation "[||-v Γ ]"                        := [ VR | ||-v Γ ] (at level 0, Γ
 Notation "[||-v Γ ≅ Γ' ]"                   := [ VR | ||-v Γ ≅ Γ' ] (at level 0, Γ, Γ' at level 50).
 Notation "[ Δ ||-v σ : Γ | VΓ | wfΔ ]"      := [ VR | Δ ||-v σ : Γ | VΓ | wfΔ ]  (at level 0, Δ, σ, Γ, VΓ, wfΔ at level 50).
 Notation "[ Δ ||-v σ ≅ σ' : Γ | VΓ | wfΔ ]" := [ VR | Δ ||-v σ ≅ σ' : Γ | VΓ | wfΔ ] (at level 0, Δ, σ, σ', Γ, VΓ, wfΔ at level 50).
-Notation "[ Γ ||-v< l > A | VΓ ]"           := [ VΓ | Γ ||-v< l > A ≅ A ] (at level 0, Γ, l , A, VΓ at level 50).
-Notation "[ Γ ||-v< l > A ≅ B | VΓ ]"       := [ VΓ | Γ ||-v< l > A ≅ B ] (at level 0, Γ, l , A, B, VΓ at level 50).
+Notation "[ Γ ||-vS< l > A | VΓ ]"          := [ VΓ | Γ ||-vS< l > A ≅ A ] (at level 0, Γ, l , A, VΓ at level 50).
+Notation "[ Γ ||-vS< l > A ≅ B | VΓ ]"      := [ VΓ | Γ ||-vS< l > A ≅ B ] (at level 0, Γ, l , A, B, VΓ at level 50).
+Notation "[ Γ ||-v< l > A | VΓ ]"          := [ VΓ | Γ ||-v< l > A ≅ A ] (at level 0, Γ, l , A, VΓ at level 50).
+Notation "[ Γ ||-v< l > A ≅ B | VΓ ]"      := [ VΓ | Γ ||-v< l > A ≅ B ] (at level 0, Γ, l , A, B, VΓ at level 50).
 
 
 Section MoreDefs.
   Context `{ta : tag} `{WfContext ta} `{WfType ta} `{Typing ta}
   `{ConvType ta} `{ConvTerm ta} `{ConvNeuConv ta} `{RedType ta} `{RedTerm ta}.
 
-  Definition validEmpty@{i j k l} {L L'}: [VR@{i j k l}| ||-v fromFctx L ≅ fromFctx L' ] := Build_VAdequate emptyVPack VREmpty.
+  Definition validEmpty@{i j k l} {L L'} (eq : L =ε L') : [VR@{i j k l}| ||-v fromFctx L ≅ fromFctx L' ] :=
+    Build_VAdequate (emptyVPack@{k} eq) (VREmpty eq).
 
   Definition validSnoc@{i j k l} {Γ Γ' : context} {A A' l}
-    (VΓ : [VR@{i j k l}| ||-v Γ ≅ Γ']) (VA : [Γ ||-v< l > A ≅ A' | VΓ])
+    (VΓ : [VR@{i j k l}| ||-v Γ ≅ Γ']) (VA : [Γ ||-vS< l > A ≅ A' | VΓ])
     : [||-v Γ ,, A ≅ Γ' ,, A'] :=
     Build_VAdequate (snocVPack Γ Γ' VΓ A A' l VA) (VRSnoc VΓ VΓ VA).
+
+
+  Record StermEqValidity@{i j k l} {Γ Γ' : context} {l} {A A' : term}
+    {VΓ : [VR@{i j k l}| ||-v Γ ≅ Γ']}
+    {VA : StypeValidity@{k i j k l} Γ Γ' VΓ l A A' (*[Γ ||-v<l> A |VΓ]*)} {t u} : Type :=
+    {
+      SvalidTmExt : forall {Δ}(wfΔ : [|- Δ]) {σ σ'}
+         (Vσσ' : [Δ ||-v σ ≅ σ' : Γ | VΓ | wfΔ]),
+        [Δ ||-<l> t[σ] ≅ u[σ'] : A[σ] | SvalidTyExt VA wfΔ Vσσ']
+    }.
+
+  Record StmEqValidity {Γ Γ' : context} {l} {t t' A A' : term} {VΓ : [||-v Γ ≅ Γ']} : Type :=
+    {
+      SVty  : [Γ ||-vS< l > A ≅ A' | VΓ] ;
+      SVeq  : @StermEqValidity Γ Γ' l A A' VΓ SVty t t'
+    }.
+
+  Record redValidity {Γ Γ'} {t u A : term} {VΓ : [||-v Γ ≅ Γ']} : Type :=
+    {
+      validRed : forall {Δ} (wfΔ : [|- Δ]) {σ σ'} (Vσσ' : [Δ ||-v σ ≅ σ' : Γ | VΓ | wfΔ]),
+        [Δ |- t[σ] ⤳* u[σ] : A[σ]]
+    }.
+
+
 
   Record termEqValidity@{i j k l} {Γ Γ' : context} {l} {A A' : term}
     {VΓ : [VR@{i j k l}| ||-v Γ ≅ Γ']}
     {VA : typeValidity@{k i j k l} Γ Γ' VΓ l A A' (*[Γ ||-v<l> A |VΓ]*)} {t u} : Type :=
     {
-      validTmExt : forall {Δ}(wfΔ : [|- Δ]) {ρF : Γ ≤ε Δ} {ρF' : Γ' ≤ε Δ} {σ σ'}
+      validTmExt : forall {Δ}(wfΔ : [|- Δ]) {σ σ'}
          (Vσσ' : [Δ ||-v σ ≅ σ' : Γ | VΓ | wfΔ]),
         [Δ ||-<l> t[σ] ≅ u[σ'] : A[σ] | validTyExt VA wfΔ Vσσ']
     }.
-
 
   Record tmEqValidity {Γ Γ' : context} {l} {t t' A A' : term} {VΓ : [||-v Γ ≅ Γ']} : Type :=
     {
@@ -178,11 +252,8 @@ Section MoreDefs.
       Veq  : @termEqValidity Γ Γ' l A A' VΓ Vty t t'
     }.
 
-  Record redValidity {Γ Γ'} {t u A : term} {VΓ : [||-v Γ ≅ Γ']} : Type :=
-    {
-      validRed : forall {Δ} (wfΔ : [|- Δ]) {ρF : Γ ≤ε Δ} {ρF' : Γ' ≤ε Δ} {σ σ'} (Vσσ' : [Δ ||-v σ ≅ σ' : Γ | VΓ | wfΔ]),
-        [Δ |- t[σ] ⤳* u[σ] : A[σ]]
-    }.
+
+
 End MoreDefs.
 
 Arguments termEqValidity : clear implicits.
@@ -193,14 +264,38 @@ Arguments tmEqValidity : clear implicits.
 Arguments tmEqValidity {_ _ _ _ _ _ _ _ _}.
 Arguments Build_tmEqValidity {_ _ _ _ _ _ _ _ _}.
 
+Arguments StermEqValidity : clear implicits.
+Arguments StermEqValidity {_ _ _ _ _ _ _ _ _}.
+Arguments Build_StermEqValidity {_ _ _ _ _ _ _ _ _}.
+
+Arguments StmEqValidity : clear implicits.
+Arguments StmEqValidity {_ _ _ _ _ _ _ _ _}.
+Arguments Build_StmEqValidity {_ _ _ _ _ _ _ _ _}.
+
 Arguments redValidity : clear implicits.
 Arguments redValidity {_ _ _ _ _ _ _ _ _}.
 Arguments Build_redValidity {_ _ _ _ _ _ _ _ _}.
 
+Notation "[ Γ ||-vS< l > t : A | VΓ | VA ]"     := (StermEqValidity Γ _ l A _ VΓ VA t t) (at level 0, Γ, l, t, A, VΓ, VA at level 50).
+Notation "[ Γ ||-vS< l > t ≅ u : A | VΓ | VA ]" := (StermEqValidity Γ _ l A _ VΓ VA t u) (at level 0, Γ, l, t, u, A, VΓ, VA at level 50).
+Notation "[ Γ ||-vS< l > t ≅ u : A | VΓ ]"      := (StmEqValidity Γ _ l t u A _ VΓ) (at level 0, Γ, l, t, u, A, VΓ at level 50).
 Notation "[ Γ ||-v< l > t : A | VΓ | VA ]"     := (termEqValidity Γ _ l A _ VΓ VA t t) (at level 0, Γ, l, t, A, VΓ, VA at level 50).
 Notation "[ Γ ||-v< l > t ≅ u : A | VΓ | VA ]" := (termEqValidity Γ _ l A _ VΓ VA t u) (at level 0, Γ, l, t, u, A, VΓ, VA at level 50).
 Notation "[ Γ ||-v< l > t ≅ u : A | VΓ ]"      := (tmEqValidity Γ _ l t u A _ VΓ) (at level 0, Γ, l, t, u, A, VΓ at level 50).
 Notation "[ Γ ||-v t ⤳* u : A | VΓ ]"      := (redValidity Γ _ t u A VΓ) (at level 0, Γ, t, u, A, VΓ at level 50).
+
+Lemma validTm_return  `{GenericTypingProperties} {Γ Γ' l t u A B}
+  {VΓ : [VR| ||-v Γ ≅ Γ']} {VA : [Γ ||-vS< l > A ≅ B | VΓ]}:
+  [ Γ ||-vS< l > t ≅ u : A | VΓ | VA ] -> [ Γ ||-v< l > t ≅ u : A | VΓ | validTy_return VA ].
+Proof.
+  intros vtu.
+  constructor.
+  intros.
+  unshelve eapply irrLR, Wpack_return', vtu; tea.
+  now eapply WAd_return, VA.
+Qed.
+
+
 
 Section Inductions.
   Context `{ta : tag} `{WfContext ta} `{WfType ta} `{Typing ta}
@@ -208,7 +303,7 @@ Section Inductions.
 
   Theorem VR_rect
     (P : forall {Γ Γ' vSubstExt}, VR Γ Γ' vSubstExt -> Type)
-    (hε : forall {L L'}, P (VREmpty (L:=L) (L':=L')))
+    (hε : forall {L L'} (eq : L =ε L'), P (VREmpty (L:=L) (L':=L') eq))
     (hsnoc : forall {Γ Γ' A A' l VΓ VΓad VA},
       P VΓad -> P (VRSnoc (Γ := Γ) (Γ':=Γ') (A := A) (A':=A') (l := l) VΓ VΓad VA)) :
     forall {Γ Γ' : context} {vSubstExt} (VΓ : VR Γ Γ' vSubstExt), P VΓ.
@@ -218,8 +313,8 @@ Section Inductions.
 
   Theorem validity_rect
     (P : forall {Γ Γ' : context}, [||-v Γ ≅ Γ'] -> Type)
-    (hε : forall {L L'}, P validEmpty (Γ:=fromFctx L) (Γ':=fromFctx L'))
-    (hsnoc : forall {Γ Γ' : context}  {A A' l} (VΓ : [||-v Γ ≅ Γ']) (VA : [Γ ||-v< l > A ≅ A' | VΓ]), P VΓ -> P (validSnoc VΓ VA)) :
+    (hε : forall {L L'} (eq : L =ε L'), P (validEmpty eq))
+    (hsnoc : forall {Γ Γ' : context}  {A A' l} (VΓ : [||-v Γ ≅ Γ']) (VA : [Γ ||-vS< l > A ≅ A' | VΓ]), P VΓ -> P (validSnoc VΓ VA)) :
     forall {Γ Γ' : context} (VΓ : [||-v Γ ≅ Γ']), P VΓ.
   Proof.
     intros Γ Γ' [[eq] VΓad]; revert Γ Γ' eq VΓad.
@@ -233,7 +328,7 @@ Section Inductions.
 
 
   (* Example check_uip_context : UIP context. Proof. typeclasses eauto. Qed. *)
-  Lemma invValidity {Γ Γ' : context} (VΓ : [||-v Γ ≅ Γ']) :
+(*   Lemma invValidity {Γ Γ' : context} (VΓ : [||-v Γ ≅ Γ']) :
     match Γ as Γ return forall Γ', [||-v Γ ≅ Γ'] -> Type with
     | Build_context nil L => fun Γ₀ VΓ₀ => ∑ (e : Tctx Γ₀ = nil),
         rew [fun Γ₀ => [||-v fromFctx L ≅ Γ₀]] (f_equal (fun Γ => Build_context Γ (Fctx Γ₀)) e) in VΓ₀ = validEmpty
@@ -245,21 +340,40 @@ Section Inductions.
     pattern Γ, Γ', VΓ; apply validity_rect; intros.
     - exists eq_refl; reflexivity.
     - do 5 eexists; do 2 exists eq_refl; reflexivity.
+  Defined. *)
+
+  (* Example check_uip_context : UIP context. Proof. typeclasses eauto. Qed. *)
+  Lemma invValidity {Γ Γ' : context} (VΓ : [||-v Γ ≅ Γ']) :
+    match Γ as Γ return forall Γ', [||-v Γ ≅ Γ'] -> Type with
+    | Build_context nil L => fun Γ₀ VΓ₀ => ∑ (L' : Fcontext) (eq : L =ε L') (e : Γ₀ = fromFctx L'),
+        rew [fun Γ₀ => [||-v fromFctx L ≅ Γ₀]] e in VΓ₀ = (validEmpty eq)
+    | Build_context (A :: Γ)%list L => fun Γ₀ VΓ₀ =>
+      ∑ l A' Γ' (VΓ : [||-v Build_context Γ L ≅ Γ']) (VA : [Build_context Γ L ||-vS< l > A ≅ A' | VΓ]) (e : Γ₀ = (Γ' ,, A')),
+        rew [fun Γ₀ => [||-v (Build_context Γ L),,A ≅ Γ₀]] e in VΓ₀ = validSnoc VΓ VA
+    end Γ' VΓ.
+  Proof.
+    pattern Γ, Γ', VΓ; apply validity_rect; intros.
+    - eexists; exists eq, eq_refl; reflexivity.
+    - do 5 eexists; exists eq_refl; reflexivity.
   Defined.
 
-  Lemma invValidityEmpty {L L'} (VΓ : [||-v fromFctx L ≅ fromFctx L']) : VΓ = validEmpty.
+  Lemma invValidityEmpty {L L'} (VΓ : [||-v fromFctx L ≅ fromFctx L']) : ∑ eq, VΓ = (validEmpty eq).
   Proof.
-    destruct (invValidity VΓ) as [e h].
+    destruct (invValidity VΓ) as (?&?&e&h).
+    pose proof (f_equal Fctx e) as e'; cbn in e'; destruct e'.
     rewrite (uip e eq_refl) in h.
-    apply h.
+    eexists; apply h.
   Qed.
 
   Lemma invValiditySnoc {Γ Γ' A A'} (VΓ₀ : [||-v Γ ,, A ≅ Γ',, A' ]) :
-      ∑ l (VΓ : [||-v Γ ≅ Γ']) (VA : [Γ ||-v< l > A ≅ A'| VΓ]), VΓ₀ = validSnoc VΓ VA.
+      ∑ l (VΓ : [||-v Γ ≅ Γ']) (VA : [Γ ||-vS< l > A ≅ A'| VΓ]), VΓ₀ = validSnoc VΓ VA.
   Proof.
-    destruct (invValidity VΓ₀) as (l&A''&Γ''&VΓ&VA&e&eF&h).
+    destruct (invValidity VΓ₀) as (l&A''&Γ''&VΓ&VA&e&h).
     destruct Γ' as [Γ' L'], Γ'' as [Γ'' L'']; cbn in *; subst.
-    depelim e.
+    pose proof (f_equal Fctx e) as e'; cbn in e'; destruct e'.
+    pose proof (f_equal Tctx e) as e'; cbn in e'.
+    inversion e'; subst.
+    rewrite (uip e eq_refl) in h.
     now do 3 eexists.
   Qed.
 
@@ -278,21 +392,21 @@ Ltac indValid VΓ :=
   valid substitions *)
 
 Definition wfCtxOfsubstS `{GenericTypingProperties}
-  {Γ Γ' Δ : context} {wfΔ : [|- Δ]} {ρF : Γ ≤ε Δ} {ρF' : Γ' ≤ε Δ} {σ σ'} {VΓ : [||-v Γ ≅ Γ']}  :
+  {Γ Γ' Δ : context} {wfΔ : [|- Δ]} {σ σ'} {VΓ : [||-v Γ ≅ Γ']}  :
   [Δ ||-v σ ≅ σ' : Γ | VΓ | wfΔ] -> [|- Δ] := fun _ => wfΔ.
 
 Ltac instValid vσ :=
   let wfΔ := (eval unfold wfCtxOfsubstS in (wfCtxOfsubstS vσ)) in
   repeat lazymatch goal with
-  | [H : typeValidity _ _ _ _ _ _ |- _] =>
-    try (let X := fresh "R" H in pose (X := validTyExt H wfΔ vσ)) ;
+  | [H : StypeValidity _ _ _ _ _ _ |- _] =>
+    try (let X := fresh "R" H in pose (X := SvalidTyExt H wfΔ vσ)) ;
      (* TODO: should only do that if vσ : [.. |- σ ≅ σ' : ...] with σ != σ' *)
-    try (let X := fresh "Rl" H in pose (X := validTyExt H wfΔ (lrefl vσ))) ;
-    try (let X := fresh "Rr" H in pose (X := validTyExt H wfΔ (urefl vσ))) ;
+    try (let X := fresh "Rl" H in pose (X := SvalidTyExt H wfΔ (lrefl vσ))) ;
+    try (let X := fresh "Rr" H in pose (X := SvalidTyExt H wfΔ (urefl vσ))) ;
     block H
-  | [H : termEqValidity _ _ _ _ _ _ _ _ _ |- _] =>
-    try (let X := fresh "R" H in pose (X := validTmExt H wfΔ vσ)) ;
-    try (let X := fresh "Rl" H in pose (X := validTmExt H wfΔ (lrefl vσ))) ;
-    try (let X := fresh "Rr" H in pose (X := validTmExt H wfΔ (urefl vσ))) ;
+  | [H : StermEqValidity _ _ _ _ _ _ _ _ _ |- _] =>
+    try (let X := fresh "R" H in pose (X := SvalidTmExt H wfΔ vσ)) ;
+    try (let X := fresh "Rl" H in pose (X := SvalidTmExt H wfΔ (lrefl vσ))) ;
+    try (let X := fresh "Rr" H in pose (X := SvalidTmExt H wfΔ (urefl vσ))) ;
     block H
   end; unblock.
