theories/Validity/Introductions/Pi.v
@@ -13,38 +13,38 @@ Section PiValidity.
 
   Lemma validΠdom {Γ Γ' F F' G G' l}
     {VΓ : [||-v Γ ≅ Γ']}
-    (VΠ : [Γ ||-v<l> tProd F G ≅ tProd F' G' | VΓ]) :
-    [Γ ||-v<l> F ≅ F' | VΓ].
+    (VΠ : [Γ ||-vS<l> tProd F G ≅ tProd F' G' | VΓ]) :
+    [Γ ||-vS<l> F ≅ F' | VΓ].
   Proof.
     constructor; intros ? wfΔ ?? Vσ.
-    pose proof (RΠ := validTyExt VΠ wfΔ Vσ).
+    pose proof (RΠ := SvalidTyExt VΠ wfΔ Vσ).
     rewrite 2!subst_prod in RΠ.
-    now unshelve eapply (instKripke _ (normRedΠ RΠ).(PolyRed.shpRed)).
+    now unshelve eapply (SinstKripke _ (normRedΠ RΠ).(PolyRed.shpRed)).
   Qed.
 
   Lemma validΠcod {Γ Γ' F F' G G' l}
     {VΓ : [||-v Γ ≅ Γ']}
-    (VΠ : [Γ ||-v<l> tProd F G ≅ tProd F' G' | VΓ]) :
+    (VΠ : [Γ ||-vS<l> tProd F G ≅ tProd F' G' | VΓ]) :
     [Γ,, F ||-v<l> G ≅ G' | validSnoc VΓ (validΠdom VΠ)].
   Proof.
     constructor; intros ? wfΔ ?? [Vσ hd].
-    pose proof (RΠ := validTyExt VΠ wfΔ Vσ).
+    pose proof (RΠ := SvalidTyExt VΠ wfΔ Vσ).
     rewrite 2!subst_prod in RΠ.
-    generalize (instKripkeSubst (normRedΠ RΠ).(PolyRed.posRed) _ hd).
+    generalize (instKripkeSubst wfΔ (normRedΠ RΠ).(PolyRed.posRed) _ hd).
     cbn -[wk1]; now rewrite 2!eta_up_single_subst.
   Qed.
 
   Lemma substSΠ {Γ Γ' F F' G G' t u l}
     {VΓ : [||-v Γ ≅ Γ']}
-    (VΠ : [Γ ||-v<l> tProd F G ≅ tProd F' G' | VΓ])
-    (Vt : [Γ ||-v<l> t ≅ u : F | VΓ | validΠdom VΠ]) :
+    (VΠ : [Γ ||-vS<l> tProd F G ≅ tProd F' G' | VΓ])
+    (Vt : [Γ ||-vS<l> t ≅ u : F | VΓ | validΠdom VΠ]) :
     [_ ||-v<l> G[t..] ≅ G'[u..] | VΓ].
-  Proof. eapply substS ; tea; eapply validΠcod. Qed.
+  Proof. eapply substS ; tea. eapply validΠcod. Qed.
 
   Definition PiValid {l Γ Γ' F F' G G'} (VΓ : [||-v Γ ≅ Γ'])
-    (VF : [Γ ||-v< l > F ≅ F' | VΓ ])
-    (VG : [Γ ,, F ||-v< l > G ≅ G' | validSnoc VΓ VF]) :
-    [Γ ||-v< l > tProd F G ≅ tProd F' G' | VΓ].
+    (VF : [Γ ||-vS< l > F ≅ F' | VΓ ])
+    (VG : [Γ ,, F ||-vS< l > G ≅ G' | validSnoc VΓ VF]) :
+    [Γ ||-vS< l > tProd F G ≅ tProd F' G' | VΓ].
   Proof.
     constructor; intros; rewrite 2!subst_prod.
     eapply LRPi', substParamRedTy; tea; intros; gtyping.
@@ -53,19 +53,19 @@ Section PiValidity.
 
   Lemma PiValidU {Γ Γ' F F' G G'}
     (VΓ : [||-v Γ ≅ Γ'])
-    (VF : [ Γ ||-v< one > F ≅ F' | VΓ ])
+    (VF : [ Γ ||-vS< one > F ≅ F' | VΓ ])
     (VΓF := validSnoc VΓ VF)
-    (VU : [ Γ ||-v< one > U | VΓ ])
-    (VU' : [ Γ ,, F ||-v< one > U | VΓF ])
-    (VFU : [ Γ ||-v< one > F ≅ F' : U | VΓ | VU ])
-    (VGU : [ Γ ,, F ||-v< one > G ≅ G' : U | VΓF | VU' ]) :
-    [ Γ ||-v< one > tProd F G ≅ tProd F' G' : U | VΓ | UValid VΓ ].
+    (VU : [ Γ ||-vS< one > U | VΓ ])
+    (VU' : [ Γ ,, F ||-vS< one > U | VΓF ])
+    (VFU : [ Γ ||-vS< one > F ≅ F' : U | VΓ | VU ])
+    (VGU : [ Γ ,, F ||-vS< one > G ≅ G' : U | VΓF | VU' ]) :
+    [ Γ ||-vS< one > tProd F G ≅ tProd F' G' : U | VΓ | UValid VΓ ].
   Proof.
     constructor; intros ? wfΔ0 ?? Vσ.
     pose proof (univValid zero VFU) as VF0.
     pose proof (univValid zero VGU) as VG0.
     pose (v := validSnoc VΓ (urefl VF)).
-    assert [_ ||-v<one> G ≅ G' : _ | _ | UValid v] by irrValid.
+    assert [_ ||-vS<one> G ≅ G' : _ | _ | UValid v] by irrValid.
     pose proof (Vuσ := liftSubst' VF Vσ).
     pose proof (Vuσ' := liftSubst' (urefl VF) (urefl Vσ)).
     instValid Vuσ'.
@@ -73,8 +73,8 @@ Section PiValidity.
     unshelve econstructor.
     1,2: econstructor; [apply redtmwf_refl; cbn; eapply ty_prod; tea| constructor].
     1: cbn in *; gtyping.
-    enough (h : [ Δ ||-< zero > (tProd F G)[σ] ≅ (tProd F' G')[σ']]) by exact (cumLR h).
-    eapply validTyExt; tea; unshelve eapply PiValid; tea.
+    enough (h : [ Δ ||-S< zero > (tProd F G)[σ] ≅ (tProd F' G')[σ']]) by exact (cumLR h).
+    eapply SvalidTyExt; tea; unshelve eapply PiValid; tea.
     eapply convValidTy; exact VG0.
   Qed.
 
