theories/Validity/Introductions/Sigma.v
@@ -1,5 +1,5 @@
 From Stdlib Require Import ssrbool CRelationClasses.
-From LogRel Require Import Utils Syntax.All GenericTyping LogicalRelation.
+From LogRel Require Import Utils Syntax.All GenericTyping Monad LogicalRelation.
 From LogRel.LogicalRelation Require Import Properties.
 From LogRel.LogicalRelation.Introductions Require Import Universe Poly Sigma.
 From LogRel.Validity Require Import Validity Irrelevance Properties Universe Poly ValidityTactics.
@@ -14,46 +14,46 @@ Context `{GenericTypingProperties}.
 
 Lemma validΣdom {Γ Γ' F F' G G' l}
   {VΓ : [||-v Γ ≅ Γ']}
-  (VΣ : [Γ ||-v<l> tSig F G ≅ tSig F' G' | VΓ]) :
-  [Γ ||-v<l> F ≅ F' | VΓ].
+  (VΣ : [Γ ||-vS<l> tSig F G ≅ tSig F' G' | VΓ]) :
+  [Γ ||-vS<l> F ≅ F' | VΓ].
 Proof.
-  constructor; intros ? wfΔ ?? Vσ; eapply redΣdom, (validTyExt VΣ wfΔ Vσ).
+  constructor; intros ? wfΔ ?? Vσ; eapply SredΣdom, (SvalidTyExt VΣ wfΔ Vσ).
 Qed.
 
 Lemma validΣcod {Γ Γ' F F' G G' l}
   {VΓ : [||-v Γ ≅ Γ']}
-  (VΣ : [Γ ||-v<l> tSig F G ≅ tSig F' G' | VΓ]) :
+  (VΣ : [Γ ||-vS<l> tSig F G ≅ tSig F' G' | VΓ]) :
   [Γ,, F ||-v<l> G ≅ G' | validSnoc VΓ (validΣdom VΣ)].
 Proof.
   constructor; intros ? wfΔ ?? [Vσ hd].
-  pose proof (RΠ := validTyExt VΣ wfΔ Vσ).
+  pose proof (RΠ := SvalidTyExt VΣ wfΔ Vσ).
   rewrite 2!subst_sig in RΠ.
-  generalize (instKripkeSubst (normRedΣ RΠ).(PolyRed.posRed) _ hd).
+  generalize (instKripkeSubst wfΔ (normRedΣ RΠ).(PolyRed.posRed) _ hd).
   cbn -[wk1]; now rewrite 2!eta_up_single_subst.
 Qed.
 
 Lemma substSΣ {Γ Γ' F F' G G' t u l}
   {VΓ : [||-v Γ ≅ Γ']}
-  (VΣ : [Γ ||-v<l> tSig F G ≅ tSig F' G' | VΓ])
-  (Vt : [Γ ||-v<l> t ≅ u : F | VΓ | validΣdom VΣ]) :
+  (VΣ : [Γ ||-vS<l> tSig F G ≅ tSig F' G' | VΓ])
+  (Vt : [Γ ||-vS<l> t ≅ u : F | VΓ | validΣdom VΣ]) :
   [_ ||-v<l> G[t..] ≅ G'[u..] | VΓ].
 Proof. eapply substS ; tea; eapply validΣcod. Qed.
 
 Lemma SigRed {Γ Γ' F G F' G' l}
   (VΓ : [||-v Γ ≅ Γ'])
-  (VF : [ Γ ||-v< l > F ≅ F' | VΓ ])
-  (VG : [ Γ ,, F ||-v< l > G ≅ G' | validSnoc VΓ VF ])
+  (VF : [ Γ ||-vS< l > F ≅ F' | VΓ ])
+  (VG : [ Γ ,, F ||-vS< l > G ≅ G' | validSnoc VΓ VF ])
   {Δ σ σ'} (wfΔ : [ |-[ ta ] Δ]) (Vσ : [VΓ | Δ ||-v σ ≅ σ' : _ | wfΔ])
-  : [ Δ ||-< l > (tSig F G)[σ] ≅ (tSig F' G')[σ'] ].
+  : [ Δ ||-S< l > (tSig F G)[σ] ≅ (tSig F' G')[σ'] ].
 Proof.
   rewrite 2!subst_sig; eapply LRSig', substParamRedTy; tea; intros; gtyping.
 Qed.
 
 Lemma SigValid {Γ Γ' F G F' G' l}
   (VΓ : [||-v Γ ≅ Γ'])
-  (VF : [ Γ ||-v< l > F ≅ F' | VΓ ])
-  (VG : [ Γ ,, F ||-v< l > G ≅ G' | validSnoc VΓ VF ])
-  : [Γ ||-v< l > tSig F G ≅ tSig F' G' | VΓ].
+  (VF : [ Γ ||-vS< l > F ≅ F' | VΓ ])
+  (VG : [ Γ ,, F ||-vS< l > G ≅ G' | validSnoc VΓ VF ])
+  : [Γ ||-vS< l > tSig F G ≅ tSig F' G' | VΓ].
 Proof. constructor; intros; now eapply SigRed. Qed.
 End SigmaCongRed.
 
@@ -63,10 +63,10 @@ Section SigTmValidity.
 
   Section Lemmas.
   Context {Γ Γ' F  F' G  G'} {VΓ : [||-v Γ ≅ Γ']}
-    {VF : [ Γ ||-v< one > F ≅ F' | VΓ ]}
-    (VU : [ Γ ,, F ||-v< one > U | validSnoc VΓ VF ])
-    (VFeqU : [ Γ ||-v< one > F ≅ F' : U | VΓ | UValid VΓ ])
-    (VGeqU : [ Γ ,, F ||-v< one > G ≅ G' : U | validSnoc VΓ VF | VU ]).
+    {VF : [ Γ ||-vS< one > F ≅ F' | VΓ ]}
+    (VU : [ Γ ,, F ||-vS< one > U | validSnoc VΓ VF ])
+    (VFeqU : [ Γ ||-vS< one > F ≅ F' : U | VΓ | UValid VΓ ])
+    (VGeqU : [ Γ ,, F ||-vS< one > G ≅ G' : U | validSnoc VΓ VF | VU ]).
 
 
   Lemma sigTmEq {Δ σ σ'} (tΔ : [ |-[ ta ] Δ])
@@ -90,13 +90,13 @@ Section SigTmValidity.
   End Lemmas.
 
   Context {Γ Γ' F  F' G  G'} {VΓ : [||-v Γ ≅ Γ']}
-    {VF : [ Γ ||-v< one > F ≅ F' | VΓ ]}
-    {VU : [ Γ ,, F ||-v< one > U | validSnoc VΓ VF ]}
-    (VFU : [ Γ ||-v< one > F ≅ F' : U | VΓ | UValid VΓ ])
-    (VGU : [ Γ ,, F ||-v< one > G ≅ G' : U | validSnoc VΓ VF | VU ]).
+    {VF : [ Γ ||-vS< one > F ≅ F' | VΓ ]}
+    {VU : [ Γ ,, F ||-vS< one > U | validSnoc VΓ VF ]}
+    (VFU : [ Γ ||-vS< one > F ≅ F' : U | VΓ | UValid VΓ ])
+    (VGU : [ Γ ,, F ||-vS< one > G ≅ G' : U | validSnoc VΓ VF | VU ]).
 
   Lemma SigRedU {Δ σ σ'} (tΔ : [ |-[ ta ] Δ]) (Vσ : [VΓ | Δ ||-v σ ≅ σ' : _ | tΔ])
-    : [ Δ ||-< one > (tSig F G)[σ] ≅ (tSig F' G')[σ'] : U | validTyExt (UValid VΓ) tΔ Vσ ].
+    : [ Δ ||-S< one > (tSig F G)[σ] ≅ (tSig F' G')[σ'] : U | SvalidTyExt (UValid VΓ) tΔ Vσ ].
   Proof.
     set (RΣ := SigURedTm VU VFU VGU tΔ Vσ).
     pose (v := validSnoc VΓ (urefl VF)).
@@ -109,7 +109,7 @@ Section SigTmValidity.
       eapply UValid.
   Qed.
 
-  Lemma SigValidU : [ Γ ||-v< one > tSig F G ≅ tSig F' G' : U | VΓ | UValid VΓ ].
+  Lemma SigValidU : [ Γ ||-vS< one > tSig F G ≅ tSig F' G' : U | VΓ | UValid VΓ ].
   Proof. econstructor; intros Δ tΔ  σ σ' Vσσ'; eapply SigRedU. Qed.
 
 End SigTmValidity.
@@ -119,28 +119,28 @@ Section ProjRed.
   Context `{GenericTypingProperties}.
 
   Context {l Γ Γ' F F' G G' } (VΓ : [||-v Γ ≅ Γ'])
-    (VF : [Γ ||-v< l > F ≅ F' | VΓ ])
-    (VG : [Γ ,, F ||-v< l > G ≅ G' | validSnoc VΓ VF])
+    (VF : [Γ ||-vS< l > F ≅ F' | VΓ ])
+    (VG : [Γ ,, F ||-vS< l > G ≅ G' | validSnoc VΓ VF])
     (VΣ := SigValid VΓ VF VG).
 
-  Lemma fstValid {p p'} (Vp : [Γ ||-v<l> p ≅ p' : _ | VΓ | VΣ]):
-    [Γ ||-v<l> tFst p ≅ tFst p' : _ | VΓ | VF].
+  Lemma fstValid {p p'} (Vp : [Γ ||-vS<l> p ≅ p' : _ | VΓ | VΣ]):
+    [Γ ||-vS<l> tFst p ≅ tFst p' : _ | VΓ | VF].
   Proof.
     constructor; intros; cbn; instValid Vσσ'.
-    (unshelve now eapply fstRed; eapply irrLR); refold; now rewrite <-?subst_sig.
+    (unshelve now eapply SfstRed; eapply SirrLR); refold; now rewrite <-?subst_sig.
   Qed.
 
   Lemma subst_fst {t σ} : tFst t[σ] = (tFst t)[σ].
   Proof. reflexivity. Qed.
 
-  Lemma sndValid {p p'} (Vp : [Γ ||-v<l> p ≅ p' : _ | VΓ | VΣ])
-    (VGfst := substS VG (fstValid Vp)) :
+  Lemma sndValid {p p'} (Vp : [Γ ||-vS<l> p ≅ p' : _ | VΓ | VΣ])
+    (VGfst := substS (validTy_return VG) (fstValid Vp)) :
     [Γ ||-v<l> tSnd p ≅ tSnd p' : _ | VΓ | VGfst].
   Proof.
-    constructor; intros; cbn; instValid Vσσ'.
-    unshelve (eapply irrLREq; [|now eapply sndRed, irrLR]); refold.
+    constructor; intros; cbn -[Wpack]; instValid Vσσ'.
+    unshelve (eapply irrLREq; [|now eapply sndRed, SirrLR]); refold.
     4: exact RVΣ.
-    + refold; now rewrite 2!subst_fst, <-2!singleSubstComm'.
+    + refold; rewrite 2!subst_fst, <-2!singleSubstComm'; eapply VGfst, Vσσ'.
     + now rewrite subst_fst, singleSubstComm'.
   Qed.
 
@@ -165,13 +165,13 @@ Section PairRed.
 
   Lemma pairFstValid {Γ Γ' A B a b l}
     (VΓ : [||-v Γ ≅ Γ'])
-    (VA : [ Γ ||-v<l> A | VΓ ])
-    (VB : [ Γ ,, A ||-v<l> B | validSnoc VΓ VA])
+    (VA : [ Γ ||-vS<l> A | VΓ ])
+    (VB : [ Γ ,, A ||-vS<l> B | validSnoc VΓ VA])
     (VΣ := SigValid VΓ VA VB)
-    (Va : [Γ ||-v<l> a : A | VΓ | VA])
-    (VBa := substS VB Va)
-    (Vb : [Γ ||-v<l> b : B[a..] | VΓ | VBa]) :
-    [Γ ||-v<l> tFst (tPair A B a b) ≅ a : _ | VΓ | VA].
+    (Va : [Γ ||-vS<l> a : A | VΓ | VA])
+    (VBa := SsubstS VB Va)
+    (Vb : [Γ ||-vS<l> b : B[a..] | VΓ | VBa]) :
+    [Γ ||-vS<l> tFst (tPair A B a b) ≅ a : _ | VΓ | VA].
   Proof.
     eapply redSubstValid; tea.
     constructor; intros; rewrite <-subst_fst, subst_pair.
@@ -182,15 +182,15 @@ Section PairRed.
 
   Lemma pairSndValid {Γ Γ' A B a b l}
     (VΓ : [||-v Γ ≅ Γ'])
-    (VA : [ Γ ||-v<l> A | VΓ ])
-    (VB : [ Γ ,, A ||-v<l> B | validSnoc VΓ VA])
+    (VA : [ Γ ||-vS<l> A | VΓ ])
+    (VB : [ Γ ,, A ||-vS<l> B | validSnoc VΓ VA])
     (VΣ := SigValid VΓ VA VB)
-    (Va : [Γ ||-v<l> a : A | VΓ | VA])
-    (VBa := substS VB Va)
-    (Vb : [Γ ||-v<l> b : B[a..] | VΓ | VBa])
+    (Va : [Γ ||-vS<l> a : A | VΓ | VA])
+    (VBa := SsubstS VB Va)
+    (Vb : [Γ ||-vS<l> b : B[a..] | VΓ | VBa])
     (Vfstall := pairFstValid VΓ VA VB Va Vb)
-    (VBfst := substS VB Vfstall) :
-    [Γ ||-v<l> tSnd (tPair A B a b) ≅ b : _ | VΓ | VBfst].
+    (VBfst := SsubstS VB Vfstall) :
+    [Γ ||-vS<l> tSnd (tPair A B a b) ≅ b : _ | VΓ | VBfst].
   Proof.
     eapply redSubstValid; cycle 1.
     + irrValid.
@@ -204,72 +204,225 @@ Section PairRed.
 
   Lemma pairCongValid {Γ Γ' A A' B B' a a' b b' l}
     (VΓ : [||-v Γ ≅ Γ'])
-    (VA : [ Γ ||-v<l> A ≅ A' | VΓ ])
-    (VB : [ Γ ,, A ||-v<l> B ≅ B' | validSnoc VΓ VA])
+    (VA : [ Γ ||-vS<l> A ≅ A' | VΓ ])
+    (VB : [ Γ ,, A ||-vS<l> B ≅ B' | validSnoc VΓ VA])
     (VΣ := SigValid VΓ VA VB)
-    (Va : [Γ ||-v<l> a ≅ a' : A | VΓ | VA])
-    (VBa := substS VB Va)
-    (Vb : [Γ ||-v<l> b ≅ b' : B[a..] | VΓ | VBa]) :
-    [Γ ||-v<l> tPair A B a b ≅ tPair A' B' a' b' : _ | VΓ | VΣ].
+    (Va : [Γ ||-vS<l> a ≅ a' : A | VΓ | VA])
+    (VBa := SsubstS VB Va)
+    (Vb : [Γ ||-vS<l> b ≅ b' : B[a..] | VΓ | VBa]) :
+    [Γ ||-vS<l> tPair A B a b ≅ tPair A' B' a' b' : _ | VΓ | VΣ].
   Proof.
     constructor; intros; rewrite 2!subst_pair.
     instValid Vσσ'; instValid (liftSubst' VA Vσσ').
-    eapply irrLREq; [now rewrite subst_sig|].
+    eapply SirrLREq; [now rewrite subst_sig|].
     eapply pairCongRed; tea.
-    now eapply irrLRConv; tea; rewrite up_subst_single'; eapply lrefl.
+    now eapply irrLRConv, Wpack_return; tea; rewrite up_subst_single'; eapply lrefl, WAd_return.
     Unshelve.
     1: now rewrite <-2!subst_sig.
-    now rewrite 2!up_subst_single'.
+    1: easy.
+    rewrite 2!up_subst_single'.
+    now eapply WAd_return.
   Qed.
 
   Lemma pairValid {Γ Γ' A A' B B' a a' b b' l}
     (VΓ : [||-v Γ ≅ Γ'])
-    (VA : [ Γ ||-v<l> A ≅ A' | VΓ ])
-    (VB : [ Γ ,, A ||-v<l> B ≅ B' | validSnoc VΓ VA])
+    (VA : [ Γ ||-vS<l> A ≅ A' | VΓ ])
+    (VB : [ Γ ,, A ||-vS<l> B ≅ B' | validSnoc VΓ VA])
     (VΣ := SigValid VΓ VA VB)
-    (Va : [Γ ||-v<l> a ≅ a' : A | VΓ | VA])
-    (VBa := substS VB Va)
-    (Vb : [Γ ||-v<l> b ≅ b' : B[a..] | VΓ | VBa]) :
-    [Γ ||-v<l> tPair A B a b : _ | VΓ | VΣ].
+    (Va : [Γ ||-vS<l> a ≅ a' : A | VΓ | VA])
+    (VBa := SsubstS VB Va)
+    (Vb : [Γ ||-vS<l> b ≅ b' : B[a..] | VΓ | VBa]) :
+    [Γ ||-vS<l> tPair A B a b : _ | VΓ | VΣ].
   Proof. now eapply lrefl, pairCongValid. Qed.
 
-  Lemma sigEtaEqValid {Γ A B p p' l}
+  Lemma SsigEtaEqValid {Γ A B p p' l}
     (VΓ : [||-v Γ])
-    (VA : [ Γ ||-v<l> A | VΓ ])
-    (VB : [ Γ ,, A ||-v<l> B | validSnoc VΓ VA])
+    (VA : [ Γ ||-vS<l> A | VΓ ])
+    (VB : [ Γ ,, A ||-vS<l> B | validSnoc VΓ VA])
     (VΣ := SigValid VΓ VA VB)
-    (Vp : [Γ ||-v<l> p : _ | VΓ | VΣ])
-    (Vp' : [Γ ||-v<l> p' : _ | VΓ | VΣ])
-    (Vfstpp' : [Γ ||-v<l> tFst p ≅ tFst p' : _ | VΓ | VA])
+    (Vp : [Γ ||-vS<l> p : _ | VΓ | VΣ])
+    (Vp' : [Γ ||-vS<l> p' : _ | VΓ | VΣ])
+    (Vfstpp' : [Γ ||-vS<l> tFst p ≅ tFst p' : _ | VΓ | VA])
     (Vfst := fstValid VΓ VA VB Vp)
-    (VBfst := substS VB Vfst)
-    (Vsndpp' : [Γ ||-v<l> tSnd p ≅ tSnd p' : _| VΓ | VBfst]) :
-    [Γ ||-v<l> p ≅ p' : _ | VΓ | VΣ].
+    (VBfst := SsubstS VB Vfst)
+    (Vsndpp' : [Γ ||-vS<l> tSnd p ≅ tSnd p' : _| VΓ | VBfst]) :
+    [Γ ||-vS<l> p ≅ p' : _ | VΓ | VΣ].
   Proof.
     constructor; intros.
-    pose proof (substS VB Vfstpp').
+    pose proof (SsubstS VB Vfstpp').
     instValid Vσσ'.
-    eapply irrLREq; [now rewrite subst_sig|].
+    eapply SirrLREq; [now rewrite subst_sig|].
     eapply sigEtaRed.
-    + now eapply lrefl, irrLR.
-    + now eapply urefl, irrLR.
+    + now eapply lrefl, SirrLR.
+    + now eapply urefl, SirrLR.
     + tea.
     + eapply irrLREq; tea.
       now rewrite subst_fst, up_subst_single'.
     Unshelve.
     2: now erewrite <-2!subst_sig.
-    now rewrite 2!subst_fst, 2!up_subst_single'.
+    unshelve now eapply Wpack_return.
+    1:easy.
+    rewrite 2!subst_fst, 2!up_subst_single'.
+    now eapply WAd_return.
+  Qed.
+
+  Lemma FequivValid {Γ Γ' : context} (VΓ : [||-v Γ ≅ Γ']) : Γ =ε Γ'.
+  Proof.
+    induction Γ, Γ', VΓ using validity_rect; tea.
+  Qed.
+
+(*   Lemma FSnocValidTy {Γ} {new} A . *)
+
+  Lemma validFSnoc {Γ Γ' : context} (VΓ : [||-v Γ ≅ Γ']) {new : newnat Γ} {new' : newnat Γ'} {b}:
+    new = new' :> nat -> [||-v Γ,, new ↦ b ≅ Γ',, new' ↦ b].
+  Proof.
+    intros.
+    induction Γ, Γ', VΓ using validity_rect.
+    + eapply validEmpty, Fequiv_Fup; now symmetry.
+    + change [||-v Γ,, new ↦ b,,A ≅ Γ',, new' ↦ b,,A'].
+      eapply validSnoc.
+      constructor.
+      intros * h.
+      eapply (wkValidTy (wk_Fstep (new : newnat Γ) b wk_id)) in VA.
+      rewrite 2!wk_Fstep_ren_on,  2!wk_id_ren_on in VA.
+      eapply VA, h.
+      Unshelve.
+      easy.
+  Defined.
+
+  Lemma irrSubstEq {Γ0 Γ0' Γ1 Γ1'} {VΓ0 : [||-v Γ0 ≅ Γ0']} {VΓ1 : [||-v Γ1 ≅ Γ1']} :
+    Γ0 = Γ1 ->
+    forall {Δ} (wfΔ : [|- Δ]) {σ σ'},
+    [Δ ||-v σ ≅ σ' : _ | VΓ0 | wfΔ ] ->
+    [Δ ||-v σ ≅ σ' : _ | VΓ1 | wfΔ ].
+  Proof.
+    intros <- *.
+    eapply convSubst.
+  Qed.
+
+  Lemma validFSnocSubst_in {Γ Γ' : context} (VΓ : [||-v Γ ≅ Γ']) {new : newnat Γ} {new' : newnat Γ'} {b σ σ'} {Δ wfΔ}
+    ( e: new = new' :> nat) :
+    [Δ ||-v σ ≅ σ' : _ | VΓ | wfΔ] -> in_Fctx Δ new b -> [Δ ||-v σ  ≅ σ' : Γ,, new ↦ b | validFSnoc VΓ e | wfΔ].
+  Proof.
+    revert σ σ'.
+    induction Γ, Γ', VΓ using validity_rect; intros σ σ' [] hin.
+    + constructor.
+      now eapply Fwk_new.
+    + econstructor.
+      now eapply SirrLR.
+      Unshelve.
+      now unshelve now eapply irrelevanceSubst, IHVΓ.
+  Qed.
+
+  Lemma FSnocSubst {Γ Γ' : context} (VΓ : [||-v Γ ≅ Γ']) :
+  forall {σ σ' Δ new b} (wfΔ : [|- Δ]) (wfΔnew : [|- Δ,, new ↦ b]),
+  [Δ ||-v σ ≅ σ' : Γ | VΓ | wfΔ ] ->
+  [Δ,,new ↦ b ||-v σ ≅ σ' : Γ | VΓ | wfΔnew ].
+  Proof.
+    intros ???????. revert σ σ'.
+    induction Γ, Γ', VΓ using validity_rect; intros ?? [].
+    + constructor.
+      now eapply Fwk_Fstep.
+    + unshelve econstructor.
+      now eapply IHVΓ.
+      eapply (SirrLREq (A:= A[↑ >> σ]⟨wk_Fstep new b wk_id⟩)).
+      etransitivity; [eapply wk_Fstep_ren_on | eapply wk_id_ren_on].
+      rewrite <- (wk_id_ren_on Δ (σ var_zero)), <- (wk_id_ren_on Δ (σ' var_zero)),
+        <- 2(wk_Fstep_ren_on new b).
+      eapply SwkLR, eqHead.
+      Unshelve.
+      now eapply wfc_consF.
+  Qed.
+
+  Lemma validFSnocSubst_notin {Γ Γ' : context} (VΓ : [||-v Γ ≅ Γ']) {new : newnat Γ} {new' : newnat Γ'} {b σ σ'} {Δ wfΔ}
+    ( e: new = new' :> nat) (Vσσ' : [Δ ||-v σ ≅ σ' : _ | VΓ | wfΔ]) (notinΔ : not_in_Fctx Δ new) :
+      let newΔ := Build_newnat Δ new notinΔ in [Δ,,newΔ ↦ b ||-v σ  ≅ σ' : Γ,, new ↦ b | validFSnoc VΓ e | wfc_consF wfΔ].
+  Proof.
+    intros ?.
+    eapply validFSnocSubst_in.
+    now eapply FSnocSubst.
+    cbn.
+    eapply in_hereF.
+  Qed.
+
+  Lemma validTy_shf {Γ} {wfΓ : [|-Γ]} {VΓ : [||-v Γ]} {l A B} :
+    shf wfΓ (fun Δ wfΔ ρ => forall (VΔ : [||-v Δ]), [Δ ||-v< l > A⟨ρ⟩ ≅ B⟨ρ⟩ | VΔ]).
+  Proof.
+    intros ???? ht hf ?.
+(*     set (new' := Build_newnat Δ' new (wk_new_notin new (lFwk (FequivValid VΔ)))). *)
+    specialize (ht (validFSnoc VΔ eq_refl)).
+    specialize (hf (validFSnoc VΔ eq_refl)).
+    rewrite 2 !wk_Fstep_ren_on in ht,hf.
+    constructor.
+    intros Ξ wfΞ ???.
+    destruct (decide_in Ξ new) as [ [] hin | hnotin].
+    - eapply ht.
+      eapply validFSnocSubst_in; tea.
+    - eapply hf.
+      eapply validFSnocSubst_in; tea.
+    - eapply WAd_split.
+      + eapply ht.
+        now unshelve eapply validFSnocSubst_notin, vσσ'.
+      + eapply hf.
+        now unshelve eapply validFSnocSubst_notin, vσσ'.
+  Qed.
+
+  Lemma Split_bind_validTy {Γ} {wfΓ : [|-Γ]} {VΓ : [||-v Γ]} {l A B C } (hC : Split (wfΓ:=wfΓ) C) :
+    (forall Δ (VΔ : [||-v Δ]) (ρ : Δ ≤ Γ), overtree hC Δ -> [Δ ||-v< l > A⟨ρ⟩ ≅ B⟨ρ⟩ | VΔ]) ->
+    [Γ ||-v< l > A ≅ B | VΓ].
+  Proof.
+    intros hAB.
+    rewrite <- (wk_id_ren_on Γ A), <- (wk_id_ren_on Γ B).
+    unshelve eapply (Split_bind_alg validTy_shf hC), wfΓ; tea.
+    intros ??? ohC ?.
+    now eapply hAB.
+  Qed.
+
+
+  Lemma sigEtaEqValid {Γ A B p p' l}
+    (VΓ : [||-v Γ])
+    (VA : [ Γ ||-vS<l> A | VΓ ])
+    (VB : [ Γ ,, A ||-vS<l> B | validSnoc VΓ VA])
+    (VΣ := SigValid VΓ VA VB)
+    (Vp : [Γ ||-vS<l> p : _ | VΓ | VΣ])
+    (Vp' : [Γ ||-vS<l> p' : _ | VΓ | VΣ])
+    (Vfstpp' : [Γ ||-vS<l> tFst p ≅ tFst p' : _ | VΓ | VA])
+    (Vfst := fstValid VΓ VA VB Vp)
+    (VBfst := substS (validTy_return VB) Vfst)
+    (Vsndpp' : [Γ ||-v<l> tSnd p ≅ tSnd p' : _| VΓ | VBfst]) :
+    [Γ ||-v<l> p ≅ p' : _ | VΓ | validTy_return VΣ].
+  Proof.
+    constructor.
+    intros.
+    eapply (dSplit_bind_return (Vsndpp'.(validTmExt) _ Vσσ')).
+    intros Ξ wfΞ ρΞ oVBfst oVsndpp' oVΣ.
+    rewrite 2!subst_ren_wk.
+    eapply (SirrLREq (A:= (tSig A B)[σ⟨ρΞ⟩])).
+    1: symmetry; eapply subst_ren_wk.
+    eapply SsigEtaEqValid.
+    1: eapply irrValidTm, Vp'; eapply VΣ.
+    1: eapply Vfstpp'.
+    constructor.
+    intros Θ wfΘ τ τ' Vττ'.
+    eapply SirrLR.
+    pose proof (Vsndpp'.(validTmExt) _ 
+    1: irrValid.
+    change (subst_term (σ >> ren_term ρΞ) p) with (p[σ >> ren_term ρΞ]).
+    Search "subst" "ren". concl:( _[_]⟨_⟩ ). ren1
   Qed.
 
 
   Lemma sigEtaValid {Γ A B p l}
     (VΓ : [||-v Γ])
-    (VA : [ Γ ||-v<l> A | VΓ ])
-    (VB : [ Γ ,, A ||-v<l> B | validSnoc VΓ VA])
+    (VA : [ Γ ||-vS<l> A | VΓ ])
+    (VB : [ Γ ,, A ||-vS<l> B | validSnoc VΓ VA])
     (VΣ := SigValid VΓ VA VB)
-    (Vp : [Γ ||-v<l> p : _ | VΓ | VΣ]) :
-    [Γ ||-v<l> tPair A B (tFst p) (tSnd p) ≅ p : _ | VΓ | VΣ].
+    (Vp : [Γ ||-vS<l> p : _ | VΓ | VΣ]) :
+    [Γ ||-v<l> tPair A B (tFst p) (tSnd p) ≅ p : _ | VΓ | validTy_return VΣ].
   Proof.
+    eapply sigEtaEqValid.
+    + irrValid.
+    + eapply pairFstValid.
     pose (Vfst := fstValid _ _ _ Vp).
     pose (Vsnd := sndValid _ _ _ Vp).
     pose proof (pairFstValid _ _ _ Vfst Vsnd).
