theories/Validity/Irrelevance.v
@@ -15,26 +15,16 @@ Universes u1 u2 u3 u4 v1 v2 v3 v4.
 
 Set Printing Universes.
 Lemma VRirrelevant@{} (Γ Γ':context) 
-  {veqsubst : forall Δ (h :[|-Δ]) {ρF : Γ ≤ε Δ} {ρF' : Γ' ≤ε Δ} (σ σ' : nat -> term), Type@{u3}}
-  {veqsubst' : forall Δ (h :[|-Δ]) {ρF : Γ ≤ε Δ} {ρF' : Γ' ≤ε Δ} (σ σ' : nat -> term), Type@{v3}}
+  {veqsubst : forall Δ (h :[|-Δ]) (σ σ' : nat -> term), Type@{u3}}
+  {veqsubst' : forall Δ (h :[|-Δ]) (σ σ' : nat -> term), Type@{v3}}
   (vr : VR@{u1 u2 u3 u4} Γ Γ' veqsubst) (vr' : VR@{v1 v2 v3 v4} Γ Γ'  veqsubst') :
-  (forall (Δ:context) wfΔ wfΔ' {ρF : Γ ≤ε Δ} {ρF' : Γ' ≤ε Δ} σ σ', veqsubst Δ wfΔ σ σ' <~> veqsubst' Δ wfΔ' σ σ').
+  (forall (Δ:context) wfΔ wfΔ' σ σ', veqsubst Δ wfΔ σ σ' <~> veqsubst' Δ wfΔ' σ σ').
 Proof.
   revert veqsubst' vr'. pattern Γ, Γ', veqsubst, vr.
   apply VR_rect; clear Γ Γ' veqsubst vr.
   - intros * h. inversion h; subst.
-    apply Specif.eq_sigT_uncurried_iff in H11; cbn in H11; destruct H11 as [eL e'].
-    assert (eq_refl = eL) as eeL by apply uip; destruct eeL; cbn in *.
-    apply Specif.eq_sigT_uncurried_iff in e'; cbn in e'; destruct e' as [eL' e].
-    assert (eq_refl = eL') as eeL' by apply uip; destruct eeL' ; cbn in *.
-    destruct e.
-    intros; split; intros; constructor.
+    intros; split; intros []; now constructor.
   - intros [Γ L] [Γ' L'] ?????? ih ? h; inversion h as [|?????? VΓad' VA' ]; subst.
-    apply Specif.eq_sigT_uncurried_iff in H18; cbn in H18; destruct H18 as [eΓA e'].
-    assert (eq_refl = eΓA) as eeΓA by apply uip; destruct eeΓA; cbn in *.
-    apply Specif.eq_sigT_uncurried_iff in e'; cbn in e'; destruct e' as [eΓA' e].
-    assert (eq_refl = eΓA') as eeΓA' by apply uip; destruct eeΓA' ; cbn in *.
-    destruct e.
     specialize (ih _ VΓad').
     intros; split; intros []; unshelve econstructor.
     1,2: now eapply ih.
@@ -53,7 +43,7 @@ Succeed Constraint v4 < u4.
 End VRIrrelevant.
 
 
-Lemma irrelevanceSubst {Γ Γ'} (VΓ VΓ' : [||-v Γ ≅ Γ']) {Δ} (wfΔ wfΔ' : [|- Δ]) {ρF : Γ ≤ε Δ} {ρF' : Γ' ≤ε Δ} {σ σ'}:
+Lemma irrelevanceSubst {Γ Γ'} (VΓ VΓ' : [||-v Γ ≅ Γ']) {Δ} (wfΔ wfΔ' : [|- Δ]) {σ σ'}:
   [Δ ||-v σ ≅ σ' : Γ | VΓ | wfΔ ] -> [Δ ||-v σ ≅ σ' : Γ | VΓ' | wfΔ'].
 Proof.
   eapply VRirrelevant; eapply VAd.adequate.
@@ -64,49 +54,52 @@ Lemma symSubst@{u1 u2 u3 u4} {Γ Γ'}
                      (VΓ  : VAdequate@{u3 u4} VR@{u1 u2 u3 u4} Γ Γ')
                      (VΓ'  : VAdequate@{u3 u4} VR@{u1 u2 u3 u4} Γ' Γ) :
   (* (VΓ VΓ' : [||-v Γ]) : *)
-  forall {Δ} (wfΔ wfΔ' : [|- Δ]) {ρF : Γ ≤ε Δ} {ρF' : Γ' ≤ε Δ} {σ σ'},
+  forall {Δ} (wfΔ wfΔ' : [|- Δ]) {σ σ'},
   [Δ ||-v σ ≅ σ' : Γ | VΓ | wfΔ ] -> [Δ ||-v σ' ≅ σ : _ | VΓ' | wfΔ'].
 Proof.
   revert VΓ'; induction Γ, Γ', VΓ using validity_rect; intros VΓ'.
-  - rewrite (invValidityEmpty VΓ'). constructor.
+  - pose proof (invValidityEmpty VΓ') as ([]&->).
+    intros * []; constructor; tea.
+    now eapply Fwk_compose.
   - pose proof (x := invValiditySnoc VΓ').
     destruct x as [lA'[ VΓ'' [VA' ->]]].
-    intros ??????? [tleq hdeq].
-    pose (tleq' := IHVΓ VΓ'' _ wfΔ wfΔ' _ _ _ _ tleq).
+    intros ????? [tleq hdeq].
+    pose (tleq' := IHVΓ VΓ'' _ wfΔ wfΔ' _ _ tleq).
     exists tleq'; now eapply symLR, SirrLR.
 Qed.
 
 Lemma symValidTy {Γ Γ' l A B} {VΓ : [||-v Γ ≅ Γ']} (VΓ' : [||-v Γ' ≅ Γ]) :
-  [Γ ||-v<l> A ≅ B | VΓ] -> [Γ' ||-v<l> B ≅ A | VΓ'].
+  [Γ ||-vS<l> A ≅ B | VΓ] -> [Γ' ||-vS<l> B ≅ A | VΓ'].
 Proof.
   intros; constructor; intros; symmetry.
-  now unshelve (eapply (validTyExt (Γ:=Γ) (Γ':=Γ')); tea; now eapply symSubst).
+  now unshelve (eapply (SvalidTyExt (Γ:=Γ) (Γ':=Γ')); tea; now eapply symSubst).
 Qed.
 
 Lemma symValid {Γ Γ'} : [||-v Γ ≅ Γ'] -> [||-v Γ' ≅ Γ].
 Proof.
   intros VΓ; induction Γ, Γ', VΓ using validity_rect.
-  - apply validEmpty.
+  - apply validEmpty; now symmetry.
   - now eapply (validSnoc IHVΓ), symValidTy.
 Qed.
 
 
 Lemma convSubst {Γ Γ' Γ''}
   (VΓ : [||-v Γ ≅ Γ']) (VΓ' : [||-v Γ ≅ Γ'']) :
-  forall {Δ} (wfΔ : [|- Δ]) {ρF : Γ ≤ε Δ} {ρF' : Γ' ≤ε Δ} {ρF' : Γ'' ≤ε Δ} {σ σ'},
+  forall {Δ} (wfΔ : [|- Δ]) {σ σ'},
   [Δ ||-v σ ≅ σ' : _ | VΓ | wfΔ ] ->
   [Δ ||-v σ ≅ σ' : _ | VΓ' | wfΔ ].
 Proof.
   revert Γ' VΓ; indValid VΓ'.
-  - constructor.
-  - intros * ih [Γ'' L''] VΓ0 *; pose proof (invValidity VΓ0) as (?&?&?&?&?&e&eF&h); cbn in e,eF; subst; cbn in h; subst.
-    intros [tl hd]; pose proof (tl' := ih _ _ _ _ _ _ _ _ _ tl).
+  - intros *. pose proof (invValidity VΓ) as (?&?&e&h); subst; cbn in h; subst.
+    intros []; now constructor.
+  - intros * ih *. pose proof (invValidity VΓ0) as (?&?&?&?&?&e&h); subst; cbn in h; subst.
+    intros [tl hd]; pose proof (tl' := ih _ _ _ _ _ _ tl).
     exists tl'; now eapply SirrLREqCum.
 Qed.
 
 Lemma convSubst' {Γ Γ' Γ''}
   (VΓ : [||-v Γ' ≅ Γ]) (VΓ' : [||-v Γ'' ≅ Γ]) :
-  forall {Δ} (wfΔ : [|- Δ]) {ρF : Γ ≤ε Δ} {ρF' : Γ' ≤ε Δ} {ρF' : Γ'' ≤ε Δ} {σ σ'},
+  forall {Δ} (wfΔ : [|- Δ]) {σ σ'},
   [Δ ||-v σ ≅ σ' : _ | VΓ' | wfΔ ] ->
   [Δ ||-v σ ≅ σ' : _ | VΓ | wfΔ ].
 Proof.
@@ -116,14 +109,14 @@ Qed.
 
 Lemma convValidTy {Γ Γ' Γ''}
   (VΓ' : [||-v Γ ≅ Γ']) (VΓ'' : [||-v Γ ≅ Γ'']) {l A B} :
-  [_ ||-v<l> A ≅ B | VΓ'] -> [_ ||-v<l> A ≅ B | VΓ''].
-Proof. intros VA; constructor. intros. eapply (validTyExt (Γ:=Γ) (Γ':=Γ')); tea; now eapply convSubst.
+  [_ ||-vS<l> A ≅ B | VΓ'] -> [_ ||-vS<l> A ≅ B | VΓ''].
+Proof. intros VA; constructor. intros. eapply (SvalidTyExt (Γ:=Γ) (Γ':=Γ')); tea; now eapply convSubst.
   Unshelve.
 Qed.
 
 Lemma convValidTy' {Γ Γ' Γ''}
   (VΓ : [||-v Γ ≅ Γ']) (VΓ' : [||-v Γ'' ≅ Γ']) {l A B} :
-  [_ ||-v<l> A ≅ B | VΓ] -> [_ ||-v<l> A ≅ B | VΓ'].
+  [_ ||-vS<l> A ≅ B | VΓ] -> [_ ||-vS<l> A ≅ B | VΓ'].
 Proof.
   intros ?%(symValidTy (symValid VΓ)).
   unshelve now eapply symValidTy, convValidTy.
@@ -139,38 +132,39 @@ Lemma transSubst {Γ Γ' Γ''}
     [Δ ||-v σ ≅ σ'' : _ | VΓ'' | wfΔ ].
 Proof.
   revert  Γ' VΓ VΓ'; indValid VΓ''.
-  - constructor.
-  - intros ????? VΓ VA ih ? VΓ0'.
-    pose proof (invValidity VΓ0') as (?&?&?&?&?&e&?); subst; cbn in *.
+  - intros *. pose proof (invValidity VΓ) as (?&?&e&h); subst; cbn in h; subst.
+    intros [] _; now constructor.
+  - intros ????? VΓ VA ih ? VΓ'0.
+    pose proof (invValidity VΓ'0) as (?&?&?&?&?&e&?); subst; cbn in *.
     intros VΓ'; pose proof (invValiditySnoc VΓ') as (?&?&?&?); subst.
     intros ???? wfΔ [tl hd] [tl' hd'].
     pose (tl'' := ih _ _ _ _ _ _ _ _ tl tl').
-    exists tl''; etransitivity; [now eapply irrLR|].
-    eapply irrLRCum; tea; symmetry; now eapply validTyExt.
+    exists tl''; etransitivity; [now eapply SirrLR|].
+    eapply SirrLRCum; tea; symmetry; now eapply SvalidTyExt.
 Qed.
 
 Lemma ureflValidTy {Γ Γ' l A B} (VΓ : [||-v Γ ≅ Γ']) (VΓ' : [||-v Γ' ≅ Γ']) :
-  [Γ ||-v<l> A ≅ B | VΓ] -> [Γ' ||-v<l> B ≅ B | VΓ'].
+  [Γ ||-vS<l> A ≅ B | VΓ] -> [Γ' ||-vS<l> B ≅ B | VΓ'].
 Proof.
   constructor; intros; etransitivity.
-  2: eapply validTyExt; tea; now eapply convSubst'.
-  symmetry; eapply validTyExt; tea.
+  2: eapply SvalidTyExt; tea; now eapply convSubst'.
+  symmetry; eapply SvalidTyExt; tea.
   unshelve eapply convSubst'; [| tea|].
   unshelve (eapply transSubst; tea; now eapply symSubst); tea.
 Qed.
 
 Lemma ureflValid {Γ Γ'} (VΓ : [||-v Γ ≅ Γ']) : [||-v Γ' ≅ Γ'].
 Proof.
-  indValid VΓ; [apply validEmpty|].
+  indValid VΓ; [intros; eapply validEmpty; reflexivity|].
   intros ????? ? VA ih; eapply (validSnoc ih).
   now eapply ureflValidTy.
 Qed.
 
 Lemma irrLvlValidTy {Γ Γ' l l' A B C} (VΓ : [||-v Γ ≅ Γ']) :
-  [Γ ||-v<l> A ≅ B | VΓ ] -> [Γ ||-v<l'> B ≅ C | VΓ] -> [Γ ||-v<l> B ≅ C | VΓ].
+  [Γ ||-vS<l> A ≅ B | VΓ ] -> [Γ ||-vS<l'> B ≅ C | VΓ] -> [Γ ||-vS<l> B ≅ C | VΓ].
 Proof.
   constructor; intros.
-  eapply transLR; [eapply urefl|];  eapply validTyExt; tea.
+  eapply transLR; [eapply urefl|];  eapply SvalidTyExt; tea.
   unshelve (eapply transSubst; [|eapply convSubst, symSubst]; tea).
   2: now eapply symValid.
   now eapply ureflValid.
@@ -178,9 +172,9 @@ Qed.
 
 Lemma transValidTy {Γ Γ' Γ'' l l' A B C}
   (VΓ : [||-v Γ ≅ Γ']) (VΓ' : [||-v Γ' ≅ Γ'']) (VΓ'' : [||-v Γ ≅ Γ'']) :
-  [Γ ||-v<l> A ≅ B | VΓ ] -> [Γ' ||-v<l'> B ≅ C | VΓ'] -> [Γ ||-v<l> A ≅ C | VΓ''].
+  [Γ ||-vS<l> A ≅ B | VΓ ] -> [Γ' ||-vS<l'> B ≅ C | VΓ'] -> [Γ ||-vS<l> A ≅ C | VΓ''].
 Proof.
-  constructor; intros; etransitivity; eapply validTyExt; tea.
+  constructor; intros; etransitivity; eapply SvalidTyExt; tea.
   2: eapply irrLvlValidTy; [now eapply convValidTy|now eapply convValidTy'].
   eapply transSubst; tea.
   unshelve now eapply convSubst, symSubst.
@@ -191,7 +185,9 @@ Qed.
 Lemma transValid {Γ Γ' Γ''} : [||-v Γ ≅ Γ'] -> [||-v Γ' ≅ Γ''] -> [||-v Γ ≅ Γ''].
 Proof.
   intros VΓ; revert Γ''; indValid VΓ.
-  - easy.
+  - intros ???? VL'.
+    pose proof (invValidity VL') as (?&?&e&?); subst; cbn in *; subst.
+    eapply validEmpty; now etransitivity.
   - intros * VA ih ? VΓ0.
     pose proof (invValidity VΓ0) as (?&?&?&VΓ'&?&e&?); subst; cbn in *; subst.
      eapply (validSnoc (ih _ VΓ')), transValidTy; tea.
@@ -212,7 +208,7 @@ Proof.
     now eapply urefl.
 Qed.
 
-Instance perValidTy {Γ Γ' l} (VΓ : [||-v Γ ≅ Γ']) : PER (typeValidity _ _ VΓ l).
+Instance perValidTy {Γ Γ' l} (VΓ : [||-v Γ ≅ Γ']) : PER (StypeValidity _ _ VΓ l).
 Proof.
   constructor; red; intros.
   - unshelve now eapply symValidTy, convValidTy, convValidTy'.
@@ -221,7 +217,7 @@ Proof.
     now eapply urefl.
 Qed.
 
-Instance iperValidTy l : IPER (VAdequate VR) (fun _ => term) (fun _ _ VΓ => typeValidity _ _ VΓ l).
+Instance iperValidTy l : IPER (VAdequate VR) (fun _ => term) (fun _ _ VΓ => StypeValidity _ _ VΓ l).
 Proof.
   constructor.
   - intros; now eapply symValidTy.
@@ -241,7 +237,7 @@ Qed.
 Lemma irrValidTy  {Γ0 Γ0' Γ1 Γ1' l A B}
   {VΓ0 : [||-v Γ0 ≅ Γ0']}
   {VΓ1 : [||-v Γ1 ≅ Γ1']}
-  : [||-v Γ0 ≅ Γ1] -> [Γ0 ||-v<l> A ≅ B | VΓ0] -> [Γ1 ||-v<l> A ≅ B | VΓ1].
+  : [||-v Γ0 ≅ Γ1] -> [Γ0 ||-vS<l> A ≅ B | VΓ0] -> [Γ1 ||-vS<l> A ≅ B | VΓ1].
 Proof.
   intros; unshelve now eapply convValidTy, convValidTy'.
   etransitivity; [|tea]; now symmetry.
@@ -249,22 +245,22 @@ Qed.
 
 Lemma irrValidTyRfl {Γ Γ' l A B}
   {VΓ VΓ' : [||-v Γ ≅ Γ']}
-  : [Γ ||-v<l> A ≅ B | VΓ] -> [Γ ||-v<l> A ≅ B | VΓ'].
+  : [Γ ||-vS<l> A ≅ B | VΓ] -> [Γ ||-vS<l> A ≅ B | VΓ'].
 Proof.
   eapply irrValidTy; now eapply lrefl.
 Qed.
 
 Lemma symValidTy' {Γ Γ' l A B} {VΓ : [||-v Γ ≅ Γ']} :
-  [_ ||-v<l> A ≅ B | VΓ] -> [_ ||-v<l> B ≅ A | symValid VΓ].
+  [_ ||-vS<l> A ≅ B | VΓ] -> [_ ||-vS<l> B ≅ A | symValid VΓ].
 Proof. eapply symValidTy. Qed.
 
 
 
 (* Still useful ?*)
 Lemma irrelevanceLift {l A F G Γ} (VΓ : [||-v Γ])
-  (VFG : [Γ ||-v<l> F ≅ G | VΓ]) :
-  [Γ ,, F ||-v<l> A | validSnoc VΓ VFG] ->
-  [Γ ,, G ||-v<l> A | validSnoc VΓ (symmetry VFG)].
+  (VFG : [Γ ||-vS<l> F ≅ G | VΓ]) :
+  [Γ ,, F ||-vS<l> A | validSnoc VΓ VFG] ->
+  [Γ ,, G ||-vS<l> A | validSnoc VΓ (symmetry VFG)].
 Proof.
   intros; eapply irrValidTy; tea; now eapply validSnoc.
 Qed.
@@ -273,27 +269,27 @@ Lemma irrValidTm {Γ0 Γ0' Γ1 Γ1' l l0 l1 A0 A0' A1 A1' t u}
   {VΓ0 : [||-v Γ0 ≅ Γ0']}
   {VΓ1 : [||-v Γ1 ≅ Γ1']}
   (VΓ01 : [||-v Γ0 ≅ Γ1])
-  (VA0 : [_ ||-v<l0> A0 ≅ A0' | VΓ0])
-  (VA1 : [_ ||-v<l1> A1 ≅ A1' | VΓ1]) :
-  [_ ||-v<l> A0 ≅ A1 | VΓ01] ->
-  [_ ||-v<l0> t ≅ u : _ | _ | VA0] ->
-  [_ ||-v<l1> t ≅ u :  _ | _ | VA1].
+  (VA0 : [_ ||-vS<l0> A0 ≅ A0' | VΓ0])
+  (VA1 : [_ ||-vS<l1> A1 ≅ A1' | VΓ1]) :
+  [_ ||-vS<l> A0 ≅ A1 | VΓ01] ->
+  [_ ||-vS<l0> t ≅ u : _ | _ | VA0] ->
+  [_ ||-vS<l1> t ≅ u :  _ | _ | VA1].
 Proof.
   intros VA Vt; constructor; intros.
   assert [VΓ0 | _ ||-v σ ≅ σ' : _ | wfΔ]
   by (eapply irrSubst; tea; now symmetry).
-  eapply irrLRCum.
-  2: now unshelve now eapply validTmExt.
-  eapply validTyExt; tea.
+  eapply SirrLRCum.
+  2: now unshelve now eapply SvalidTmExt.
+  eapply SvalidTyExt; tea.
   now eapply lrefl, convSubst.
 Qed.
 
 Lemma irrValidTmRfl {Γ Γ' l A A' B B' t u}
   {VΓ VΓ' : [||-v Γ ≅ Γ']}
-  {VA : [Γ ||-v<l> A ≅ B | VΓ]}
-  {VA' : [Γ ||-v<l> A' ≅ B' | VΓ']} :
+  {VA : [Γ ||-vS<l> A ≅ B | VΓ]}
+  {VA' : [Γ ||-vS<l> A' ≅ B' | VΓ']} :
   A = A' ->
-  [_ ||-v<l> t ≅ u : _ | _ | VA] -> [_ ||-v<l> t ≅ u : _ | _ | VA'].
+  [_ ||-vS<l> t ≅ u : _ | _ | VA] -> [_ ||-vS<l> t ≅ u : _ | _ | VA'].
 Proof.
   intros ?; subst.
   unshelve now eapply irrValidTm; eapply convValidTy; eapply lrefl.
@@ -301,34 +297,34 @@ Proof.
 Qed.
 
 
-Instance perValidTm {Γ Γ' l A A'} (VΓ : [||-v Γ ≅ Γ']) (VA : [_ ||-v<l> A ≅ A' | VΓ]) :
-  PER (termEqValidity _ _ _ _ _ VΓ VA).
+Instance perValidTm {Γ Γ' l A A'} (VΓ : [||-v Γ ≅ Γ']) (VA : [_ ||-vS<l> A ≅ A' | VΓ]) :
+  PER (StermEqValidity _ _ _ _ _ VΓ VA).
 Proof.
   constructor; red; intros; constructor; intros.
-  - eapply symLR, irrLRConv.
-    2: (unshelve now eapply validTmExt) ; tea; now symmetry.
-    eapply validTyExt; tea; now eapply urefl.
-  - unshelve now etransitivity; eapply irrLR; eapply validTmExt.
+  - eapply symLR, SirrLRConv.
+    2: (unshelve now eapply SvalidTmExt) ; tea; now symmetry.
+    eapply SvalidTyExt; tea; now eapply urefl.
+  - unshelve now etransitivity; eapply SirrLR; eapply SvalidTmExt.
     all: first [eassumption | now eapply lrefl].
 Qed.
 
 Lemma symValidTm {Γ Γ' l A A' t t'}
   {VΓ : [||-v Γ ≅ Γ']} (VΓ' : [||-v Γ' ≅ Γ])
-  {VA : [Γ ||-v<l> A ≅ A' | VΓ]} (VA' : [_ ||-v<l> A' ≅ A | VΓ']) :
-  [_ ||-v<l> t ≅ t' : _ | _ | VA] -> [_ ||-v<l> t' ≅ t : _ | _ | VA'].
+  {VA : [Γ ||-vS<l> A ≅ A' | VΓ]} (VA' : [_ ||-vS<l> A' ≅ A | VΓ']) :
+  [_ ||-vS<l> t ≅ t' : _ | _ | VA] -> [_ ||-vS<l> t' ≅ t : _ | _ | VA'].
 Proof. intros; symmetry; now eapply irrValidTm. Qed.
 
 Lemma symValidTm' {Γ Γ' l A A' t t'}
-  {VΓ : [||-v Γ ≅ Γ']} {VA : [_ ||-v<l> A ≅ A' | VΓ]} :
-  [_ ||-v<l> t ≅ t' : _ | _ | VA] -> [_ ||-v<l> t' ≅ t : _ | _ | symValidTy' VA ].
+  {VΓ : [||-v Γ ≅ Γ']} {VA : [_ ||-vS<l> A ≅ A' | VΓ]} :
+  [_ ||-vS<l> t ≅ t' : _ | _ | VA] -> [_ ||-vS<l> t' ≅ t : _ | _ | symValidTy' VA ].
 Proof. now apply symValidTm. Qed.
 
 Lemma transValidTm {Γ Γ' Γ'' l A A' A'' t t' t''}
   {VΓ : [||-v Γ ≅ Γ']} (VΓ' : [||-v Γ' ≅ Γ'']) (VΓ'' : [||-v Γ ≅ Γ''])
-  {VA : [Γ ||-v<l> A ≅ A' | VΓ]} (VA' : [_ ||-v<l> A' ≅ A'' | VΓ']) (VA'' : [_ ||-v<l> A ≅ A'' | VΓ'']) :
-  [_ ||-v<l> t ≅ t' : _ | _ | VA] ->
-  [_ ||-v<l> t' ≅ t'' : _ | _ | VA'] ->
-  [_ ||-v<l> t ≅ t'' : _ | _ | VA''].
+  {VA : [Γ ||-vS<l> A ≅ A' | VΓ]} (VA' : [_ ||-vS<l> A' ≅ A'' | VΓ']) (VA'' : [_ ||-vS<l> A ≅ A'' | VΓ'']) :
+  [_ ||-vS<l> t ≅ t' : _ | _ | VA] ->
+  [_ ||-vS<l> t' ≅ t'' : _ | _ | VA'] ->
+  [_ ||-vS<l> t ≅ t'' : _ | _ | VA''].
 Proof.
   intros; etransitivity; eapply irrValidTm.
   2,4: tea.
@@ -344,12 +340,12 @@ Lemma irrelevanceSubstEqExt {Γ Γ'} (VΓ : [||-v Γ ≅ Γ']) {σ1 σ1' σ2 σ2
   [Δ ||-v σ1' ≅ σ2' : Γ | VΓ | wfΔ ].
 Proof.
   revert Δ wfΔ σ1 σ1' σ2 σ2' eq1 eq2; indValid VΓ.
-  - constructor.
+  - intros * ?? []. now constructor.
   - intros ??????? ih ?????? eq1 eq2 [tl hd].
     unshelve eexists (ih _ _ _ _ _ _ _ _ tl).
     1,2: red; intros; eauto.
     rewrite <- (eq1 var_zero); rewrite <- (eq2 var_zero).
-    eapply irrLREq; tea; now rewrite eq1.
+    eapply SirrLREq; tea; now rewrite eq1.
 Qed.
 
 End Irrelevances.
